% !TEX root = /Users/us2009801/Documents/GitHub/DifferentialEquations/main.tex
\chapter{Class 13 - Monday, March 20\ts{th}, 2017}
\section*{\S 22B Variation of Parameters}
Before: The method of Coefficients required $Q(x)$ to have a finite number of linearly independent derivatives.\\
Now: Allow $Q(x)$ to have any form\\
Start: Constant Coefficient 2\ts{nd} order Differential Equations: $y''+$ stuff\\
If you know two solutions, $y_1, y_2$,etc. of any $a_2y''+ a_1y'+a_0y=0$ are known, use these to find $y_p'$\\
$$y_p=u_1(x)y_1(x)+u_2(x)y_2(x)$$ where $u_1, u_2$ satisfy\\
\begin{align*}
    u_1'*y_1+u_2'*y_2&=0\\
    u_1'*y_1'+u_2'*y_2'&=\frac{Q(x)}{a_2}
\end{align*}
Helpful Identities: 
\begin{align*}
1&=\sin^2x+\cos^2x\\
\sin(2x)&=2\\
\text{Insert Stuff Here I missed it}
\end{align*}
\begin{ex}
$y''+y=\cot x$
\begin{align*}
y''+y&=\cot x\\
    m^2+1&=0\\
    m&=0 \pm 1i\\
    \alpha &=0\\
    \beta &=1\\
    y_c &= c_1\cos x + c_2 \sin x\\
    y_1&=c_1\cos x \\
    y_2&= c_2 \sin x\\
    u_1'(\cos x)+u_2'(\sin x) &= 0\\
    u_1'(\cos x)' + u_2'(\sin x)' &=\cot x\\
    u_1'(-\sin x) + u_2'(\cos x) &=\cot x
\end{align*}
$\star$ =$\left[
                \begin{array}{ll}
                  u_1'(\cos x)+u_2'(\sin x) &= 0\\
                  u_1'(-\sin x) + u_2'(\cos x) &=\cot x
                \end{array}
              \right] $\\
$\left[
                \begin{array}{ll}
                  u_1'(\cos x)+u_2'(\sin x) &= 0\\
                  u_1'(-\sin x) + u_2'(\cos x) &=\cot x
                \end{array}
              \right] *\left[
              \begin{array}{ll}
                   \cos x\\
                   \sin x
              \end{array}
              \right]
              $
\end{ex}
\begin{ex}
$y''+3y'+2y=12e^x$
\begin{align*}
    y''+3y'+2y&=12e^x\\
    m^2+3m+2&=0\\
    (m+2)(m+1)&=0\\
    m&=-2\\
    m&=-1\\
    y_c&=c_1e^{-2x}+c_2e^{-x}\\
    y_2&=e^{-2x}\\
    y_1&=e^{-x}
\end{align*}
$\star =\left\{
                \begin{array}{rcl}
                  u_1'(e^{-x})&+ u_2'(e^{-2x}) &= 0\\
                  u_1'(-e^{-x}) &+ u_2'(-2e^{-2x}) &=12e^x
                \end{array}
              \right\} $\\
            $\left\{
                \begin{array}{rcl}
                  u_1'(e^{-x})&+ u_2'(e^{-2x}) &= 0\\
                  u_1'(-e^{-x}) &+ u_2'(-2e^{-2x}) &=12e^x
                \end{array}
              \right\} * \left[
                \begin{array}{c}
                  1\\
                  1
                \end{array}
              \right] * $
\end{ex}